Using Bayes' theorem we can write

\begin{align*}
	p(\theta | x < 3) = \frac{p(x < 3 | \theta)p(\theta)}{p(x < 3)}
\end{align*}

Prior can be written as the pdf of Beta distribution = $Beta(\theta, 1, 1) = \frac{1}{Beta(1, 1)} \theta (1 - \theta)^{1- 1} = Uniform(0, 1)$ 

Further, the likelihood can be given as 
\begin{align*}
	p(x < 3 | \theta) & = \sum_{i=1}^{3}p(x = i | \theta) \\
	& = \begin{pmatrix} 5 \\ 0 \end{pmatrix}\theta^{0} (1 - \theta)^{5} + \begin{pmatrix} 5 \\ 1 \end{pmatrix}\theta^{2} (1 - \theta)^{4} + \begin{pmatrix} 5 \\ 2 \end{pmatrix}\theta^{2} (1 - \theta)^{3} \\
	& = \sum_{k=0}^{2} Binomial(k | \theta, 5)
\end{align*}

Therefor, the posterior can then be approximated as

\begin{align*}
	p(\theta | x < 3) & \approx p(x < 3 | \theta)p(\theta) \\
	& = (\sum_{k=0}^{2} Binomial(k | \theta, 5)) \cdot Uniform(0, 1)
\end{align*}