\section{Problem 7}

	\begin{align*}
		||X^{T}w - y||^{2} = \underbrace{(w - \hat{w})^{T} X^{T}X (w - \hat{w})}_{(x - M^{-1}b)^{T} x^{T}x (x - M^{-1}b)} + ||X^{T}\hat{w} - y||^{2}
	\end{align*}
	We can show that $||X^{T}w - y||^{2} - ||X^{T}\hat{w} - y||^{2} = (w - \hat{w})^{T} X^{T}X (w - \hat{w})$ 
	\par
	Let $x = w, M = X^{T}X, b = X^{T}y$. Then $(w - \hat{w})^{T} X^{T}X (w - \hat{w})$ can be written as $(x - M^{-1}b)^{T} x^{T}x (x - M^{-1}b)$. Also, we know that \\
	\begin{align*}
		(x - M^{-1}b)^{T} x^{T}x (x - M^{-1}b) = x^{T}Mx - 2b^{T}x + b^{T}M^{-1}b \\		
	\end{align*}
	Therefore
	\begin{align*}
		(w - \hat{w})^{T} X^{T}X (w - \hat{w}) & = w^{T}X^{T}Xw - 2(X^{T}y)^{T}w + (X^{T}y)^{T}(X^{T}X)^{-1}(X^{T}y) \\
		& = w^{T}X^{T}Xw - 2(X^{T}y)^{T}w + (X^{T}y)^{T}\hat{w}(X^{T}y)^{-1}(X^{T}y)
	\end{align*}
	% Next, we need to show that $||X^{T}w - y||^{2} - ||X^{T}\hat{w} - y||^{2}$ can be written as $x^{T}Mx - 2b^{T}x + b^{T}M^{-1}b$. \\
	Next,
	\begin{align*}
		||X^{T}w - y||^{2}- ||X^{T}\hat{w} - y||^{2} & = (X^{T}w)^{T}(X^{T}w) - 2y^{T}(X^{T}w) + y^{T}y - (X^{T}\hat{w})^{T}(X^{T}\hat{w}) + 2y^{T}(X^{T}\hat{w}) - y^{T}y \\
		& = (X^{T}w)^{T}(X^{T}w) - (X^{T}\hat{w})^{T}(X^{T}\hat{w}) - 2y^{T}(X^{T}w) + 2y^{T}(X^{T}\hat{w})
	\end{align*}
